Metrology/ProbLang/PureStep.lean
@@ -1,0 +1,133 @@
+import Metrology.ProbLang.PrimStep
+import Mathlib.Order.Defs.PartialOrder
+
+noncomputable section PureStep
+open Classical MeasureTheory ProbabilityTheory Measure
+
+local instance : MeasurableSpace Expr := ⊤
+local instance : MeasurableSpace State := ⊤
+local instance : MeasurableSpace Val := ⊤
+local instance : MeasurableSpace Cfg := ⊤
+
+-- Record pure_step (e1 e2 : expr Λ) := {
+--   pure_step_safe σ1 : reducible (e1, σ1);
+--   pure_step_det σ : prim_step e1 σ (e2, σ) = 1;
+-- }.
+structure PureStep (e1 e2 : Expr) : Prop where
+  safe : ∀ σ, ∃ ρ : Cfg, PrimStep ⟨e1, σ⟩ {ρ} > 0
+  det  : ∀ σ, PrimStep ⟨e1, σ⟩ {⟨e2, σ⟩} = 1
+
+-- Class PureExec (φ : Prop) (n : nat) (e1 e2 : expr Λ) :=
+--   pure_exec : φ → relations.nsteps pure_step n e1 e2.
+class PureExec (φ : Prop) (n : ℕ) (e1 e2 : Expr) : Prop where
+  pure_exec : φ → Relation.ReflTransGen PureStep e1 e2
+
+-- Record pure_head_step (e1 e2 : expr Λ) := {
+--   pure_head_step_safe σ1 : head_reducible e1 σ1;
+--   pure_head_step_det σ1 : head_step e1 σ1 (e2, σ1) = 1;
+-- }.
+structure PureHeadStep (e1 e2 : Expr) : Prop where
+  safe : ∀ σ, ∃ ρ : Cfg, HeadStep ⟨e1, σ⟩ {ρ} > 0
+  det  : ∀ σ, HeadStep ⟨e1, σ⟩ {⟨e2, σ⟩} = 1
+
+-- Lemma pure_head_step_pure_step e1 e2 : pure_head_step e1 e2 → pure_step e1 e2.
+-- Proof.
+--   intros [Hp1 Hp2]. split.
+--   - intros σ. destruct (Hp1 σ) as ([e2' σ2] & ?).
+--     eexists (e2', σ2). by apply head_prim_step.
+--   - intros σ1. rewrite /= head_prim_step_eq //.
+-- Qed.
+theorem PureHeadStep.toPureStep {e1 e2 : Expr} (h : PureHeadStep e1 e2) : PureStep e1 e2 := by
+  sorry
+
+-- Lemma pure_step_ctx K `{!@LanguageCtx Λ K} e1 e2 :
+--   pure_step e1 e2 → pure_step (K e1) (K e2).
+-- Proof.
+--   intros [Hred Hstep]. split.
+--   - unfold reducible in *. intros σ1.
+--     destruct (Hred σ1) as [[]].
+--     eexists. by eapply fill_step.
+--   - intros σ.
+--     rewrite -fill_step_prob //.
+--     eapply (to_final_None_1 (_, σ)).
+--     by eapply reducible_not_final.
+-- Qed.
+theorem PureStep.fill (K : Ectx) {e1 e2 : Expr} (h : PureStep e1 e2) :
+    PureStep (K.fill e1) (K.fill e2) := by
+  sorry
+
+-- Lemma pure_step_nsteps_ctx K `{!@LanguageCtx Λ K} n e1 e2 :
+--   relations.nsteps pure_step n e1 e2 →
+--   relations.nsteps pure_step n (K e1) (K e2).
+-- Proof. eauto using nsteps_congruence, pure_step_ctx. Qed.
+theorem PureStep.fill_nsteps (K : Ectx) {e1 e2 : Expr}
+    (h : Relation.ReflTransGen PureStep e1 e2) :
+    Relation.ReflTransGen PureStep (K.fill e1) (K.fill e2) := by
+  sorry
+
+-- Lemma pure_exec_fill K φ n e1 e2 :
+--   PureExec φ n e1 e2 →
+--   PureExec φ n (fill K e1) (fill K e2).
+-- Proof. apply: pure_exec_ctx. Qed.
+theorem PureExec.fill (K : Ectx) {φ : Prop} {n : ℕ} {e1 e2 : Expr}
+    [h : PureExec φ n e1 e2] : PureExec φ n (K.fill e1) (K.fill e2) where
+  pure_exec hφ := PureStep.fill_nsteps K (h.pure_exec hφ)
+
+-- Lemma PureExec_reducible σ1 φ n e1 e2 :
+--   φ → PureExec φ (S n) e1 e2 → reducible (e1, σ1).
+-- Proof. move => Hφ /(_ Hφ). inversion_clear 1. apply H. Qed.
+theorem PureExec.reducible {σ : State} {φ : Prop} {n : ℕ} {e1 e2 : Expr}
+    (hφ : φ) [h : PureExec φ (n + 1) e1 e2] :
+    ∃ ρ : Cfg, PrimStep ⟨e1, σ⟩ {ρ} > 0 := by
+  sorry
+
+-- Lemma PureExec_not_val `{Inhabited (language.state Λ)} φ n e1 e2 :
+--   φ → PureExec φ (S n) e1 e2 → to_val e1 = None.
+-- Proof.
+--   intros Hφ Hex.
+--   destruct (PureExec_reducible inhabitant _ _ _ _ Hφ Hex) => /=.
+--   simpl in *.
+--   by eapply val_stuck.
+-- Qed.
+theorem PureExec.not_val {φ : Prop} {n : ℕ} {e1 e2 : Expr}
+    (hφ : φ) [h : PureExec φ (n + 1) e1 e2] :
+    e1.toVal? = none := by
+  sorry
+
+-- Lemma rtc_pure_step_val `{!Inhabited (state Λ)} v e :
+--   rtc pure_step (of_val v) e → to_val e = Some v.
+-- Proof.
+--   intros ?; rewrite <- to_of_val.
+--   f_equal; symmetry; eapply rtc_nf; first done.
+--   intros [e' [Hstep _]].
+--   specialize (Hstep inhabitant) as [? Hval%val_stuck].
+--   by rewrite to_of_val in Hval.
+-- Qed.
+theorem rtc_pure_step_val {v : Val} {e : Expr}
+    (h : Relation.ReflTransGen PureStep v.1 e) :
+    e.toVal? = some v := by
+  sorry
+
+--   (* This is a family of frequent assumptions for PureExec *)
+--   Class IntoVal (e : expr Λ) (v : val Λ) :=
+--     into_val : of_val v = e.
+class IntoVal (e : Expr) (v : Val) : Prop where
+  into_val : v.1 = e
+
+--   Class AsVal (e : expr Λ) := as_val : ∃ v, of_val v = e.
+class AsVal (e : Expr) : Prop where
+  as_val : ∃ v : Val, v.1 = e
+
+--   Lemma as_val_is_Some e :
+--     (∃ v, of_val v = e) → is_Some (to_val e).
+--   Proof. intros [v <-]. rewrite to_of_val. eauto. Qed.
+theorem as_val_is_Some {e : Expr} (h : ∃ v : Val, v.1 = e) : e.isValue := by
+  sorry
+
+--   Lemma fill_is_val e K `{@LanguageCtx Λ K} :
+--     is_Some (to_val (K e)) → is_Some (to_val e).
+--   Proof. rewrite -!not_eq_None_Some. eauto using fill_not_val. Qed.
+theorem fill_is_val {K : Ectx} {e : Expr} (h : (K.fill e).isValue) : e.isValue :=
+  Ectx.fill_isValue h
+
+end PureStep
